# TD7 - Logique de Hoare II

## Règles

$$\frac{\{P\} C \{Q\} \hspace{.2cm} v_1, v_2 .. v_n \notin P \cup Q}{\{P\} \textrm{var} v_1, \textrm{var} v_2, .. , \textrm{var} v_n, C \{Q\}}\textrm{(let)}$$

$$\frac{}{\{Q[\frac{A(ex_1 \leftarrow ex_2)}{A}]\} A[ex_1] = ex_2 \{Q\}}\textrm{(tab)}$$

$$\frac{I \wedge S \Rightarrow I' \hspace{.2cm} \{I'\} C \{I\} \hspace{.2cm} I \wedge \neq S \Rightarrow Q}{\{I\} \textrm{While} \hspace{.1cm} S \hspace{.1cm} \textrm{do} \hspace{.1cm} C \{Q\}}\textrm{(while)}$$

## Ex1.

### Q1.

* Invariant:
	* Invariant
	* Vrai en entrée (et en sortie)
	
* Q: y=x
* I invariant
* $I \wedge \neg (a \neq 0) \Rightarrow (y=x)$
* $I \wedge (a = 0) \Rightarrow (y=x)$
* Invariant: x = a + y
* Variant: a

```c
{
	var a;
	a = x;
	y = 0;
	while (a != 0) {
		y = y + 1;
		a = a - 1;
		assert(x == a + y);
	}
}
```

### Q2.

$$\{x \geq 0\} Prog_1 \{x=y\}$$

1. $\{x = a - 1 + y\}a = a - 1\{x = a + y\}$(aff)
2. $\{x = a - 1 + y + 1\}y = y + 1\{x = a + y\}$(aff)
	* $\Leftrightarrow x = a + y$
3. $(x = a + y) \wedge (a \neq 0) \Rightarrow (x = a + y)$(CQFD)
4. $(x = a + y) \wedge (a = 0) \Rightarrow (x = y)$(CQFD)
5. $\{x = a + y\} ..;..;\{x = a + y\}$(seq)(2)(1)
6. $\{x = a + y\}\textrm{while} \hspace{.1cm} (a \neq 0) \hspace{.1cm} \textrm{do} \hspace{.1cm} ..\{x=y\}$(while)(3)(5)(4) -- On rajoute la contrainte du variant ici
7. $\{a \geq 0 \wedge x = a\}y=0 \{a \geq 0 \wedge x = a + y\}$(aff)
8. $\{x \geq 0 \wedge x = x\} a = x \{a \geq 0 \wedge x = a\}$(aff)
9. $\{x \geq 0 \} ..;..;.. \{x = y\}$(seq)(8)(7)(6)
10. $\{x \geq 0\}var a; ... \{x = y\}$(var)(9)

## Ex2.

1. $\{tab'[i] = y \wedge tab'[j] = x \wedge tab' = tab(j \leftarrow r)\}tab[j] = r\{tab[i] = x \wedge tab[j] = y\}$(tab)
2. $\{tab'[i] = y \wedge tab'[j] = x \wedge tab' = tab(i \leftarrow tab[j])\}tab[i] = tab[j]\{tab'[i] = x \wedge tab'[j] = y \wedge\}$(tab)
3. $\{tab'[i] = y \wedge tab'[j] = x \wedge tab' = tab(i \leftarrow tab[j])(j \leftarrow tab[i])\}r = tab[i]\{tab'[i] = y \wedge tab'[j] = x \wedge tab' = tab(i \leftarrow tab[j])(j \leftarrow r)\}$(aff)
4. $\{tab'[i] = y \wedge tab'[j] = x \wedge tab' = tab(i \leftarrow tab[j])(j \leftarrow tab[i])\} ..;..;.. \{tab[i] = y \wedge tab[j] = x\}$(seq)(3)(2)(1)
5. $\{tab'[i] = y \wedge tab'[j] = x \wedge tab' = tab(i \leftarrow tab[j])(j \leftarrow tab[i])\} var r; ... \{tab[i] = y \wedge tab[j] = x\}$(let)
 

Précondition obtenue: 

$$tab'[i] = y \wedge tab'[j] = x \wedge tab' = tab(i \leftarrow tab[j])(j \leftarrow tab[i]$$

6. $P \Rightarrow P'$(CQFD)
7. $\{P\} Prog_2 \{Q\}$(mp-pre)

## Ex3. 

* Variant : m
* Terminaison de l'invariant: $m \geq 0$
* Invariant : $x^n = y^m * p \wedge m \geq 0$

Programme:

```c
{
	var m; var y;
	m = n; p = 1; y = x;
	if (x != 0)
		while (m != 0) {
			if (odd(m)) p = p * y;
			else p = p;
			m = m div 2;
			y = y * y;
		}
	else p = 0;
}
```

### Q1.

$$\{ n \geq 0\} Prog_3 \{ p = x^n\}$$

1. $\{ x^n = 0\} p = 0 \{ p = x^n\}$(aff)
2. $\{ x^n = y^{2m} * p \wedge m \geq 0\} y =  y * y \{ x^n = y^m * p \wedge m \geq 0 \}$(aff)
3. $\{ x^n = y^{2 (m div 2)} * p \wedge m \geq 0\} m = m div 2 \{ x^n = y^{2m} * p \wedge m \geq 0\}$(aff)
4. $\{ x^n = y^{2 (m div 2)} * p \wedge m \geq 0\} p = p \{ x^n = y^{2m} * p \wedge m \geq 0\}$(aff)
5. $\{ x^n = y^{2 (m div 2) + 1} * p \wedge m \geq 0\} p = p * y \{ x^n = y^{2 (m div 2)} * p \wedge m \geq 0\}$(aff)
6. $\{ odd(m) \Rightarrow x^n = y^{2 (m div 2) + 1} * p \wedge even(m) \Rightarrow x^n = y ^{2 (m div 2)}\} if .. else .. \{ x^n = y^{2 (m div 2)} * p \wedge m \geq 0\}$(if)
